src/Assembly/GF25519.v
@@ -9,7 +9,7 @@ Module GF25519.
   Definition bits: nat := 64.
   Definition width: Width bits := W64.
 
-  Fixpoint makeBoundList {n} k (b: @WordRangeOpt n) :=
+  Fixpoint makeBoundList {n} k (b: @BoundedWord n) :=
     match k with
     | O => nil
     | S k' => cons b (makeBoundList k' b)
@@ -17,9 +17,10 @@ Module GF25519.
 
   Section DefaultBounds.
     Import ListNotations.
-    Local Notation rr exp := (makeRange 0 (2^exp + 2^exp/10)%Z).
+    Local Notation rr exp :=
+      (orElse any (make (n := bits) 0 (wzero _) (2^exp + 2^exp/10)%N)).
 
-    Definition feBound: list (@WordRangeOpt bits) :=
+    Definition feBound: list (@BoundedWord bits) :=
       [rr 26; rr 27; rr 26; rr 27; rr 26;
        rr 27; rr 26; rr 27; rr 26; rr 27].
   End DefaultBounds.
@@ -39,7 +40,7 @@ Module GF25519.
     Definition inputs: nat := 20.
     Definition width: Width bits := width.
     Definition ResultType := FE.
-    Definition inputUpperBounds: list (@WordRangeOpt bits) := feBound ++ feBound.
+    Definition inputBounds: list (@BoundedWord bits) := feBound ++ feBound.
 
     Definition ge25519_add_expr :=
         Eval cbv beta delta [fe25519 add mul sub Let_In] in add.
@@ -92,7 +93,7 @@ Module GF25519.
     Definition inputs: nat := 20.
     Definition width: Width bits := width.
     Definition ResultType := FE.
-    Definition inputUpperBounds: list (@WordRangeOpt bits) := feBound ++ feBound.
+    Definition inputBounds: list (@BoundedWord bits) := feBound ++ feBound.
 
     Definition ge25519_sub_expr :=
         Eval cbv beta delta [fe25519 add mul sub Let_In] in sub.
@@ -145,7 +146,7 @@ Module GF25519.
     Definition inputs: nat := 20.
     Definition width: Width bits := width.
     Definition ResultType := FE.
-    Definition inputUpperBounds: list (@WordRangeOpt bits) := feBound ++ feBound.
+    Definition inputBounds: list (@BoundedWord bits) := feBound ++ feBound.
 
     Definition ge25519_mul_expr :=
         Eval cbv beta delta [fe25519 add mul sub Let_In] in mul.
@@ -198,7 +199,7 @@ Module GF25519.
     Definition inputs: nat := 10.
     Definition width: Width bits := width.
     Definition ResultType := FE.
-    Definition inputUpperBounds: list (@WordRangeOpt bits) := feBound.
+    Definition inputBounds: list (@BoundedWord bits) := feBound.
 
     Definition ge25519_opp_expr :=
         Eval cbv beta delta [fe25519 add mul sub opp Let_In] in opp.
